src/Compatibility.v
@@ -95,8 +95,6 @@ Proof.
   (* TODO *)
 Abort. *)
 
-Export Coq.Arith.Wf_nat.
-
 Lemma Vrel_RecFun_compat :
   forall Γ f1 f2 vl1 vl2 b1 b2, length vl1 = length vl2 ->
   Erel_open (S (length vl1) + Γ) b1 b2 ->
